\documentclass[11pt]{article}

\usepackage{sectsty}
\usepackage{graphicx}

% Margins
\topmargin=-0.45in
\evensidemargin=0in
\oddsidemargin=0in
\textwidth=6.5in
\textheight=9.0in
\headsep=0.25in

\title{ Derivate }
\author{ Andrea Canale }
\date{\today}

\begin{document}
\maketitle	

%--Paper--
\section{Es 617 - Pag 307}

$ y_0 = x^4 - 5x^3 - 1 $

$ y_1 = 4x^3 - 15x^2 $

\section{Es 618 - Pag 307}

$ y_0 = x^3(x^2 - 1) $

$ y_1 = 3x^2(x^2 - 1) + x^3(2x) $

$ y_1 = x^2(3(x^2 - 1) + x(2x)) $

$ y_1 = x^2(3x^2 - 3 + 2x^2) $

$ y_1 = x^2(5x^2 - 3) $

\section{Es 619 - Pag 307}

$ y_0 = \frac{6}{x} - 1 $

$ y_1 = \frac{-6}{x^2} $

\section{Es 621 - Pag 307}

$ y_0 = \frac{x^2}{x + 2} $

$ y_1 = \frac{2x(x+2) - x^2(1)}{(x + 2)^2} $

$ y_1 = \frac{2x^2 + 4x - x^2}{(x + 2)^2} $

$ y_1 = \frac{x^2 + 4x}{(x + 2)^2} $

\section{Es 628 - Pag 307}

$ y_0 = e^{2x^3 - 3} $

$ y_1 = e^{2x^3 - 3} \cdot 6x^2 $

\section{Es 629 - Pag 307}

$ y_0 = x(e^{2x} - 1) $

$ y_1 = 1(e^{2x} - 1) + x(e^{2x} \cdot 2) $

$ y_1 = e^{2x} - 1 + x(e^{2x} \cdot 2) $

\section{Es 635 - Pag 307}

$ y_0 = (x^2 - 1)^3 $

$ y_1 = 3(x^2 - 1)^2 \cdot (2x)$

\section{Es 636 - Pag 307}

$ y_0 = \sin(\cos(x)) $

$ y_1 = \cos(x) \cdot -\sin(x) $

\section{Es 639 - Pag 307}

$ y_0 = (\ln(x) - x)^2 $

$ y_1 = 2(\ln(x) - x) \cdot (\frac{1}{x} - 1) $

\section{Es 640 - Pag 307}

$ y_0 = xtan^2x $

$ y_0 = x^2(\tan^2) $

$ y_0 = x^2(tan^2) $

$ y_1 = 2x(tan^2) \cdot x^2(2tan) $

$ y_1 = x(2(tan^2) + 2xtan)$


\pagebreak

\end{document}